Source/Dafny/AST/VMTPrinter.cs
@@ -1,0 +1,198 @@
+using System;
+using System.IO;
+using System.Collections.Generic;
+using System.Diagnostics.Contracts;
+using System.Numerics;
+using System.Linq;
+using System.Diagnostics;
+using Bpl = Microsoft.Boogie;
+
+namespace Microsoft.Dafny {
+  public class VMTPrinter : Printer {
+
+    private string VMT_HEADER = @"; Typecast bit to bool
+(define-sort bool_type () (_ BitVec 1))
+(define-fun bv_false () bool_type (_ bv0 1))
+(define-fun bv_true  () bool_type (_ bv1 1))
+(define-fun is_bool ((x bool_type)) Bool (or (= x bv_true) (= x bv_false))))
+";
+
+    private string STATE_MACHINE_DATATYPE_NAME = "DafnyStateMachine";
+    private string STATE_MACHINE_INIT_PRED_NAME = "Init";
+    private string STATE_MACHINE_NEXT_PRED_NAME = "Pred";
+
+    public Dictionary<System.Type, Func<Expression, string>> AstDict = new Dictionary<System.Type, Func<Expression, string>>();
+
+    public Dictionary<string, int> Instances;
+    public HashSet<int> TypeLengthSet = new HashSet<int> { 0, 1 };
+
+    public VMTPrinter(TextWriter wr,
+                      Dictionary<string, int> datatypeInstanceCounts,
+                      DafnyOptions.PrintModes printMode = DafnyOptions.PrintModes.Everything)
+        : base(wr, printMode) {
+      AstDict[typeof(BinaryExpr)] = InstantiateBinaryExpr;
+      Instances = datatypeInstanceCounts;
+    }
+
+    public override void PrintProgram(Program prog, bool afterResolver) {
+      Console.WriteLine("Creating finite instance in VMT. Datatype instance counts:");
+      Console.WriteLine(Instances);
+
+      wr.Write(VMT_HEADER);
+
+      ParseDatatypes(prog);
+      ParsePredicates(prog);
+    }
+
+    public void ParseDatatypes(Program prog) {
+      Console.WriteLine("DATATYPES");
+
+      foreach (TopLevelDecl d in prog.DefaultModuleDef.TopLevelDecls) {
+        if (d is DatatypeDecl) {
+          Console.WriteLine("DATATYPE");
+          var dd = (DatatypeDecl)d;
+          var name = dd.Name;
+
+          if (name == STATE_MACHINE_DATATYPE_NAME) {
+            // Dealing with outer state machine datatype
+          } else if (Instances.ContainsKey(name)) {
+            // Dealing with one of our finitized datatypes
+
+            var l = Convert.ToInt32(Math.Log2(Instances[name]));
+            while (TypeLengthSet.Contains(l)) {
+              l += 1;
+            }
+            TypeLengthSet.Add(l);
+            wr.WriteLine("(define-sort " + name + "_type () (_ BitVec " + l + "))");
+            var typeCheckString = "";
+            for (int i = 0; i < Instances[name]; ++i) {
+              wr.WriteLine("(define-fun " + name + i + " () " + name + "_type (_ bv" + i + " " + l + "))");
+              typeCheckString += "(= " + name + " " + name + i + ") ";
+            }
+            wr.WriteLine("(define-fun is_" + name + " ((" + name + " " + name + "_type)) Bool (or " + typeCheckString + "))");
+          } else {
+            Debug.Assert(false, "Finitized datatype '" + name + "' provided on command line but not found in Dafny program");
+          }
+          // PrintDatatype(dd, 0, Path.GetFullPath(prog.FullName));
+        }
+      }
+
+      Console.WriteLine("END DATATYPES");
+    }
+
+    public void ParsePredicates(Program prog) {
+      Console.WriteLine("PREDICATES");
+
+      foreach (TopLevelDecl d in prog.DefaultModuleDef.TopLevelDecls) {
+        if (d is ClassDecl) {
+          ClassDecl cl = (ClassDecl)d;
+          foreach (MemberDecl mem in cl.Members) {
+            if (mem is Function) {
+              Function f = (Function)mem;
+              if (f is Predicate) {
+                Console.WriteLine("PREDICATE");
+
+                ParsePredicate((Predicate)f);
+
+                // PrintFunction(f, 0, false);
+              }
+            }
+          }
+        }
+      }
+
+      Console.WriteLine("END PREDICATES");
+    }
+
+    public void ParsePredicate(Predicate pred) {
+      var name = pred.Name;
+
+      if (name == STATE_MACHINE_INIT_PRED_NAME) {
+        // Dealing with Init
+      } else if (name == STATE_MACHINE_NEXT_PRED_NAME) {
+        // Dealing with Next
+      } else {
+        // Dealing with a state transition
+      }
+    }
+
+    public string InstantiateBinaryExpr(Expression e) {
+      //assert(e is BinaryExpr);
+      Debug.Assert(e is BinaryExpr);
+      var exp = (BinaryExpr)e;
+      switch (exp.Op) {
+        case BinaryExpr.Opcode.And:
+          return InstantiateAnd(e);
+        case BinaryExpr.Opcode.Or:
+          return InstantiateOr(e);
+        case BinaryExpr.Opcode.Iff:
+          return InstantiateImplies(e);
+        case BinaryExpr.Opcode.Eq:
+          return InstantiateEqual(e);
+        case BinaryExpr.Opcode.Neq:
+          return InstantiateNotEqual(e);
+        default:
+          Console.WriteLine("unsupported binary expression: " + exp.Op);
+          break;
+      }
+      return "";
+    }
+
+    public string InstantiateAnd(Expression e) {
+      BinaryExpr exp = (BinaryExpr)e;
+      Debug.Assert(exp.Op == BinaryExpr.Opcode.And);
+      string retval = "(ite (and ";
+      retval += "(= ";
+      retval += AstDict[typeof(Expression)](exp.E0);
+      retval += " bv_true) (= ";
+      retval += AstDict[typeof(Expression)](exp.E1);
+      retval += " bv_true)) bv_true bv_false)";
+      return retval;
+    }
+
+    public string InstantiateOr(Expression e) {
+      BinaryExpr exp = (BinaryExpr)e;
+      Debug.Assert(exp.Op == BinaryExpr.Opcode.And);
+      string retval = "(ite (or (= ";
+      retval += AstDict[typeof(Expression)](exp.E0);
+      retval += " bv_true) (= ";
+      retval += AstDict[typeof(Expression)](exp.E1);
+      retval += " bv_true)) bv_true bv_false)";
+      return retval;
+    }
+
+    public string InstantiateImplies(Expression e) {
+      BinaryExpr exp = (BinaryExpr)e;
+      Debug.Assert(exp.Op == BinaryExpr.Opcode.Iff);
+      string retval = "(ite (=> (= ";
+      retval += AstDict[typeof(Expression)](exp.E0);
+      retval += " bv_true) (= ";
+      retval += AstDict[typeof(Expression)](exp.E1);
+      retval += " bv_true)) bv_true bv_false)";
+      return retval;
+    }
+
+    public string InstantiateEqual(Expression e) {
+      BinaryExpr exp = (BinaryExpr)e;
+      Debug.Assert(exp.Op == BinaryExpr.Opcode.Eq);
+      string retval = "(ite (= ";
+      retval += AstDict[typeof(Expression)](exp.E0);
+      retval += " ";
+      retval += AstDict[typeof(Expression)](exp.E1);
+      retval += ") bv_true bv_false)";
+      return retval;
+    }
+
+    public string InstantiateNotEqual(Expression e) {
+      BinaryExpr exp = (BinaryExpr)e;
+      Debug.Assert(exp.Op == BinaryExpr.Opcode.Neq);
+      string retval = "(ite (= ";
+      retval += AstDict[typeof(Expression)](exp.E0);
+      retval += " ";
+      retval += AstDict[typeof(Expression)](exp.E1);
+      retval += ") bv_false bv_true)";
+      return retval;
+    }
+  }
+
+}
